misc/miscScript.sml
@@ -3,7 +3,7 @@
    development.
 *)
 open HolKernel bossLib boolLib boolSimps lcsymtacs Parse libTheory
-open optionTheory combinTheory dep_rewrite listTheory pred_setTheory finite_mapTheory alistTheory rich_listTheory llistTheory arithmeticTheory pairTheory sortingTheory relationTheory totoTheory comparisonTheory bitTheory sptreeTheory wordsTheory wordsLib set_sepTheory indexedListsTheory stringTheory ASCIInumbersLib machine_ieeeTheory
+open bagTheory optionTheory combinTheory dep_rewrite listTheory pred_setTheory finite_mapTheory alistTheory rich_listTheory llistTheory arithmeticTheory pairTheory sortingTheory relationTheory totoTheory comparisonTheory bitTheory sptreeTheory wordsTheory wordsLib set_sepTheory indexedListsTheory stringTheory ASCIInumbersLib machine_ieeeTheory
 
 (* Misc. lemmas (without any compiler constants) *)
 val _ = new_theory "misc"
@@ -1620,6 +1620,10 @@ val FOLDL_invariant_rest = Q.store_thm("FOLDL_invariant_rest",
 val between_def = Define`
   between x y z ⇔ x:num ≤ z ∧ z < y`
 
+val IN_between = Q.store_thm("IN_between",
+  `x ∈ between y z ⇔ y ≤ x ∧ x < z`,
+  rw[IN_DEF] \\ EVAL_TAC);
+
 val SUC_LEAST = Q.store_thm("SUC_LEAST",
   `!x. P x ==> (SUC ($LEAST P) = LEAST x. 0 < x /\ P (PRE x))`,
   GEN_TAC THEN STRIP_TAC THEN
@@ -1929,6 +1933,16 @@ val lookup_vars_def = Define `
        | SOME xs => SOME (EL v env :: xs)
        | NONE => NONE
      else NONE)`
+
+val EVERY_lookup_vars = Q.store_thm(
+  "EVERY_lookup_vars",
+  `∀vs env env'. EVERY P env ∧ lookup_vars vs env = SOME env' ⇒ EVERY P env'`,
+  Induct >> simp[lookup_vars_def, CaseEq"option", CaseEq"bool", PULL_EXISTS] >>
+  metis_tac[MEM_EL, EVERY_MEM]);
+
+val EVERY_LAST = Q.store_thm("EVERY_LAST",
+  `!P l. l ≠ [] /\ EVERY P l ==> P (LAST l)`,
+  rw [LAST_EL, EVERY_EL, NOT_NIL_EQ_LENGTH_NOT_0]);
 
 val TAKE_GENLIST = Q.store_thm("TAKE_GENLIST",
   `TAKE n (GENLIST f m) = GENLIST f (MIN n m)`,
@@ -3557,5 +3571,196 @@ val FOLDL_OPTION_CHOICE_EQ_SOME_IMP_MEM = Q.store_thm("FOLDL_OPTION_CHOICE_EQ_SO
   `FOLDL OPTION_CHOICE x ls = SOME y ⇒ MEM (SOME y) (x::ls)`,
   qid_spec_tac`x` \\ Induct_on`ls` \\ rw[] \\
   res_tac \\ fs[] \\ Cases_on`x` \\ fs[]);
+
+val BAG_DISJOINT_SUB_BAG = Q.store_thm("BAG_DISJOINT_SUB_BAG",
+  `!b1 b2 b3. b1 ≤ b2 /\ BAG_DISJOINT b2 b3 ==> BAG_DISJOINT b1 b3`,
+  rw [BAG_DISJOINT_BAG_IN] \\ metis_tac [SUB_BAG, BAG_IN]);
+
+val BAG_DISJOINT_SYM = Q.store_thm("BAG_DISJOINT_SYM",
+  `!b1 b2. BAG_DISJOINT b1 b2 <=> BAG_DISJOINT b2 b1`,
+  simp [BAG_DISJOINT, DISJOINT_SYM]);
+
+val MONOID_BAG_UNION_EMPTY_BAG = Q.store_thm("MONOID_BAG_UNION_EMPTY_BAG",
+  `MONOID $⊎ {||}`,
+  simp [MONOID_DEF, RIGHT_ID_DEF, LEFT_ID_DEF, ASSOC_DEF, ASSOC_BAG_UNION]);
+
+val BAG_DISJOINT_FOLDR_BAG_UNION = Q.store_thm("BAG_DISJOINT_FOLDR_BAG_UNION",
+  `∀ls b0 b1.
+    BAG_DISJOINT b1 (FOLDR BAG_UNION b0 ls) ⇔
+    EVERY (BAG_DISJOINT b1) (b0::ls)`,
+  Induct \\ rw[] \\ metis_tac[]);
+
+val BAG_ALL_DISTINCT_FOLDR_BAG_UNION = Q.store_thm("BAG_ALL_DISTINCT_FOLDR_BAG_UNION",
+  `∀ls b0.
+   BAG_ALL_DISTINCT (FOLDR BAG_UNION b0 ls) ⇔
+   BAG_ALL_DISTINCT b0 ∧
+   (∀n. n < LENGTH ls ⇒
+        BAG_DISJOINT (EL n ls) b0 ∧ BAG_ALL_DISTINCT (EL n ls) ∧
+        (∀m. m < n ⇒ BAG_DISJOINT (EL n ls) (EL m ls)))`,
+  Induct \\ rw[]
+  \\ rw[BAG_ALL_DISTINCT_BAG_UNION]
+  \\ simp[Once FORALL_NUM, SimpRHS]
+  \\ Cases_on`BAG_ALL_DISTINCT h` \\ simp[]
+  \\ Cases_on`BAG_ALL_DISTINCT b0` \\ simp[]
+  \\ simp[BAG_DISJOINT_FOLDR_BAG_UNION, EVERY_MEM, MEM_EL, PULL_EXISTS]
+  \\ CONV_TAC(PATH_CONV"rrrarrr"(HO_REWR_CONV FORALL_NUM))
+  \\ simp[]
+  \\ rw[EQ_IMP_THM] \\ fs[]
+  \\ metis_tac[BAG_DISJOINT_SYM]);
+
+val bag_of_list_def = Define `bag_of_list = FOLDL $⊎ {||} o MAP EL_BAG`;
+
+val bag_of_list_append = Q.store_thm("bag_of_list_append",
+  `!xs ys. bag_of_list (xs ++ ys) = bag_of_list xs ⊎ bag_of_list ys`,
+  simp [bag_of_list_def, FOLDL_APPEND]
+  \\ irule COMM_MONOID_FOLDL
+  \\ simp [COMM_DEF, COMM_BAG_UNION, MONOID_BAG_UNION_EMPTY_BAG]);
+
+val bag_of_list_sub_bag_FLAT_suff = Q.store_thm("bag_of_list_sub_bag_FLAT_suff",
+  `!ls1 ls2. LIST_REL (\l1 l2. bag_of_list l1 ≤ bag_of_list l2) ls1 ls2 ==>
+     bag_of_list (FLAT ls1) ≤ bag_of_list (FLAT ls2)`,
+  ho_match_mp_tac LIST_REL_ind
+  \\ srw_tac [bagLib.SBAG_SOLVE_ss] [bag_of_list_append]);
+
+val bag_of_list_thm = Q.store_thm("bag_of_list_thm",
+  `bag_of_list [] = {||} ∧
+   (∀x xs. bag_of_list (x::xs) = BAG_INSERT x (bag_of_list xs))`,
+  conj_tac >- EVAL_TAC
+  \\ rewrite_tac[bag_of_list_def, o_DEF]
+  \\ simp_tac bool_ss []
+  \\ qmatch_goalsub_abbrev_tac`FOLDL f`
+  \\ ntac 2 gen_tac
+  \\ `COMM f` by (rw[Abbr`f`,COMM_DEF,COMM_BAG_UNION])
+  \\ `ASSOC f` by (rw[Abbr`f`,ASSOC_DEF,ASSOC_BAG_UNION])
+  \\ drule (GSYM COMM_ASSOC_FOLDL_REVERSE)
+  \\ disch_then drule
+  \\ disch_then(CONV_TAC o LAND_CONV o REWR_CONV)
+  \\ rw[FOLDL_APPEND,Abbr`f`]
+  \\ rw[COMM_ASSOC_FOLDL_REVERSE]
+  \\ rw[BAG_INSERT_UNION, COMM_BAG_UNION]);
+
+val IN_bag_of_list_MEM = Q.store_thm("IN_bag_of_list_MEM",
+  `∀l. x <: bag_of_list l ⇔ MEM x l`,
+  Induct \\ rw[bag_of_list_thm] \\ fs[]);
+
+val bag_of_list_SUB_BAG_SUBSET = Q.store_thm("bag_of_list_SUB_BAG_SUBSET",
+  `∀l1 l2. bag_of_list l1 ≤ bag_of_list l2 ⇒ set l1 ⊆ set l2`,
+  Induct \\ rw[bag_of_list_thm]
+  \\ imp_res_tac BAG_INSERT_SUB_BAG_E
+  \\ imp_res_tac IN_bag_of_list_MEM \\ fs[]);
+
+val bag_of_list_ALL_DISTINCT = Q.store_thm("bag_of_list_ALL_DISTINCT",
+  `∀ls. BAG_ALL_DISTINCT (bag_of_list ls) ⇔ ALL_DISTINCT ls`,
+  Induct \\ rw[bag_of_list_thm,IN_bag_of_list_MEM]);
+
+val is_subseq_def = Define`
+  (is_subseq ls [] ⇔ T) ∧
+  (is_subseq [] (x::xs) ⇔ F) ∧
+  (is_subseq (y::ys) (x::xs) ⇔
+   (x = y ∧ is_subseq ys xs) ∨
+   (is_subseq ys (x::xs)))`;
+
+val is_subseq_ind = theorem"is_subseq_ind";
+
+val is_subseq_refl = Q.store_thm("is_subseq_refl[simp]",
+  `∀ls. is_subseq ls ls`, Induct \\ rw[is_subseq_def]);
+
+val is_subseq_nil = Q.store_thm("is_subseq_nil[simp]",
+  `is_subseq [] ls ⇔ ls = []`,
+  Cases_on`ls` \\ rw[is_subseq_def]);
+
+val is_subseq_cons = Q.store_thm("is_subseq_cons",
+  `∀l1 l2 x. is_subseq l1 l2 ⇒ is_subseq (x::l1) l2`,
+  recInduct is_subseq_ind
+  \\ rw[is_subseq_def]);
+
+val is_subseq_snoc = Q.store_thm("is_subseq_snoc",
+  `∀l1 l2 x. is_subseq l1 l2 ⇒ is_subseq (SNOC x l1) l2`,
+  recInduct is_subseq_ind
+  \\ rw[is_subseq_def] \\ fs[]);
+
+val is_subseq_append1 = Q.store_thm("is_subseq_append1",
+  `∀l3 l1 l2. is_subseq l1 l2 ⇒ is_subseq (l3 ++ l1) l2`,
+  Induct
+  \\ rw[is_subseq_def] \\ fs[]
+  \\ metis_tac[is_subseq_cons]);
+
+val is_subseq_append2 = Q.store_thm("is_subseq_append2",
+  `∀l4 l1 l2. is_subseq l1 l2 ⇒ is_subseq (l1 ++ l4) l2`,
+  ho_match_mp_tac SNOC_INDUCT
+  \\ rw[is_subseq_def] \\ fs[]
+  \\ metis_tac[is_subseq_snoc, SNOC_APPEND, APPEND_ASSOC]);
+
+val is_subseq_IS_SUBLIST = Q.store_thm("is_subseq_IS_SUBLIST",
+  `is_subseq l1 l2 ∧ IS_SUBLIST l3 l1 ⇒ is_subseq l3 l2`,
+  rw[IS_SUBLIST_APPEND]
+  \\ metis_tac[is_subseq_append1, is_subseq_append2]);
+
+val is_subseq_MEM = Q.store_thm("is_subseq_MEM",
+  `∀l1 l2 x. is_subseq l1 l2 ∧ MEM x l2 ⇒ MEM x l1`,
+  recInduct is_subseq_ind
+  \\ rw[is_subseq_def]
+  \\ metis_tac[]);
+
+val IS_PREFIX_is_subseq = Q.store_thm("IS_PREFIX_is_subseq",
+  `∀l1 l2. IS_PREFIX l1 l2 ⇒ is_subseq l1 l2`,
+  recInduct is_subseq_ind
+  \\ rw[is_subseq_def]
+  \\ fs[IS_PREFIX_NIL]);
+
+val IS_SUBLIST_is_subseq = Q.store_thm("IS_SUBLIST_is_subseq",
+  `∀l1 l2. IS_SUBLIST l1 l2 ⇒ is_subseq l1 l2`,
+  recInduct is_subseq_ind
+  \\ rw[is_subseq_def, IS_SUBLIST]
+  \\ simp[IS_PREFIX_is_subseq]);
+
+val is_subseq_ALL_DISTINCT = Q.store_thm("is_subseq_ALL_DISTINCT",
+  `∀l1 l2. ALL_DISTINCT l1 ∧ is_subseq l1 l2 ⇒ ALL_DISTINCT l2`,
+  recInduct is_subseq_ind
+  \\ rw[is_subseq_def] \\ fs[] \\ rfs[]
+  \\ metis_tac[is_subseq_MEM]);
+
+val is_subseq_append_suff = Q.store_thm("is_subseq_append_suff",
+  `∀l1 l3 l2 l4.
+   is_subseq l1 l3 ∧ is_subseq l2 l4 ⇒
+   is_subseq (l1 ++ l2) (l3 ++ l4)`,
+  recInduct is_subseq_ind
+  \\ rw[is_subseq_def]
+  \\ metis_tac[is_subseq_append1]);
+
+val is_subseq_FLAT_suff = Q.store_thm("is_subseq_FLAT_suff",
+  `∀ls1 ls2. LIST_REL is_subseq ls1 ls2 ⇒ is_subseq (FLAT ls1) (FLAT ls2)`,
+  ho_match_mp_tac LIST_REL_ind
+  \\ rw[is_subseq_append_suff]);
+
+val LIST_REL_IMP_LAST = store_thm("LIST_REL_IMP_LAST",
+  ``!P xs ys.
+      LIST_REL P xs ys /\ (xs <> [] \/ ys <> []) ==> P (LAST xs) (LAST ys)``,
+  rpt gen_tac
+  \\ Cases_on `xs = []` \\ fs [] \\ Cases_on `ys = []` \\ fs []
+  \\ `?x1 x2. xs = SNOC x1 x2` by metis_tac [SNOC_CASES]
+  \\ `?y1 y2. ys = SNOC y1 y2` by metis_tac [SNOC_CASES]
+  \\ asm_rewrite_tac [LAST_SNOC] \\ fs [LIST_REL_SNOC]);
+
+val MAP2_APPEND = store_thm("MAP2_APPEND",
+  ``!xs ys xs1 ys1 f.
+      LENGTH xs = LENGTH xs1 ==>
+      MAP2 f (xs ++ ys) (xs1 ++ ys1) = MAP2 f xs xs1 ++ MAP2 f ys ys1``,
+  Induct \\ Cases_on `xs1` \\ fs [MAP2]);
+
+val make_even_def = Define`
+  make_even n = if EVEN n then n else n+1`;
+
+val ALOOKUP_MAP_FST_INJ_SOME = Q.store_thm("ALOOKUP_MAP_FST_INJ_SOME",
+  `∀ls x y.
+    ALOOKUP ls x = SOME y ∧ (∀x'. IS_SOME (ALOOKUP ls x') ∧ f x' = f x ⇒ x = x') ⇒
+    ALOOKUP (MAP (f ## g) ls) (f x) = SOME (g y)`,
+  Induct \\ simp[]
+  \\ Cases \\ rw[]
+  >- metis_tac[IS_SOME_EXISTS]
+  \\ first_x_assum irule
+  \\ rw[]
+  \\ first_x_assum irule
+  \\ rw[]);
 
 val _ = export_theory()
